iris/ZZprint.v
@@ -1,0 +1,6 @@
+Require Import SpecDevintr UartTxInv ConsoleInv TicksInv SpecClockintr DiskInv.
+About UartTxInv.uart_dlab_off.
+About DiskInv.disk_cfg.
+About TicksInv.is_tickslock.
+About SpecClockintr.tick_keeper.
+About ConsoleInv.cons_res_at.
