iris/ZZq.v
@@ -1,0 +1,2 @@
+Require Import SpecClockintr.
+About SpecClockintr.tick_keeper.
